tll

theories/dyn_ctx.v
@@ -40,25 +40,93 @@ Reserved Notation "Δ ▷ s" (at level 40).
 Inductive key : dyn_ctx -> sort -> Prop :=
 | key_nil s :
   nil ▷ s
-| key_u Γ m :
-  Γ ▷ U ->
-  m :U Γ ▷ U
-| key_l Γ m s :
-  Γ ▷ L ->
-  m :{s} Γ ▷ L
-| key_n Γ s :
-  Γ ▷ s ->
-  _: Γ ▷ s
-where "Γ ▷ s" := (key Γ s).
+| key_u Δ m :
+  Δ ▷ U ->
+  m :U Δ ▷ U
+| key_l Δ m s :
+  Δ ▷ L ->
+  m :{s} Δ ▷ L
+| key_n Δ s :
+  Δ ▷ s ->
+  _: Δ ▷ s
+where "Δ ▷ s" := (key Δ s).
 
 Inductive dyn_has : dyn_ctx -> var -> term -> Prop :=
-| dyn_has_O Γ A s :
-  Γ ▷ U ->
-  dyn_has (A :{s} Γ) 0 A.[ren (+1)]
-| dyn_has_S Γ A B x :
-  dyn_has Γ x A ->
-  dyn_has (B :U Γ) x.+1 A.[ren (+1)]
-| dyn_has_N Γ A x :
-  dyn_has Γ x A ->
-  dyn_has (_: Γ) x.+1 A.[ren (+1)].
+| dyn_has_O Δ A s :
+  Δ ▷ U ->
+  dyn_has (A :{s} Δ) 0 A.[ren (+1)]
+| dyn_has_S Δ A B x :
+  dyn_has Δ x A ->
+  dyn_has (B :U Δ) x.+1 A.[ren (+1)]
+| dyn_has_N Δ A x :
+  dyn_has Δ x A ->
+  dyn_has (_: Δ) x.+1 A.[ren (+1)].
 
+Lemma key_impure Δ : Δ ▷ L.
+Proof with eauto using key.
+  elim: Δ... move=>[[A s]|] Δ k...
+Qed.
+
+Lemma key_merge Δ1 Δ2 Δ s : Δ1 ∘ Δ2 => Δ -> Δ1 ▷ s -> Δ2 ▷ s -> Δ ▷ s.
+Proof with eauto using key.
+  move=>mrg. elim: mrg s=>{Δ1 Δ2 Δ}...
+  { move=>Δ1 Δ2 Δ m mrg ih s k1 k2. inv k1; inv k2... }
+  { move=>Δ1 Δ2 Δ m mrg ih s k1 k2. inv k1; inv k2... }
+  { move=>Δ1 Δ2 Δ m mrg ih s k1 k2. inv k1; inv k2... }
+  { move=>Δ1 Δ2 Δ m mrg ih k1 k2. inv k1; inv k2... }
+Qed.
+
+Lemma merge_sym Δ1 Δ2 Δ : Δ1 ∘ Δ2 => Δ -> Δ2 ∘ Δ1 => Δ.
+Proof with eauto using merge. elim... Qed.
+
+Lemma merge_pureL Δ1 Δ2 Δ : Δ1 ∘ Δ2 => Δ -> Δ1 ▷ U -> Δ = Δ2.
+Proof.
+  elim=>//={Δ1 Δ2 Δ}.
+  { move=>Δ1 Δ2 Δ m mrg ih k. inv k. by rewrite ih. }
+  { move=>Δ1 Δ2 Δ m mrg ih k. inv k. }
+  { move=>Δ1 Δ2 Δ m mrg ih k. inv k. by rewrite ih. }
+  { move=>Δ1 Δ2 Δ mrg ih k. inv k. by rewrite ih. }
+Qed.
+
+Lemma merge_pureR Δ1 Δ2 Δ : Δ1 ∘ Δ2 => Δ -> Δ2 ▷ U -> Δ = Δ1.
+Proof.
+  elim=>//={Δ1 Δ2 Δ}.
+  { move=>Δ1 Δ2 Δ m mrg ih k. inv k. by rewrite ih. }
+  { move=>Δ1 Δ2 Δ m mrg ih k. inv k. by rewrite ih. }
+  { move=>Δ1 Δ2 Δ m mrg ih k. inv k. }
+  { move=>Δ1 Δ2 Δ mrg ih k. inv k. by rewrite ih. }
+Qed.
+
+Lemma merge_splitL Δ1 Δ2 Δ Δa Δb :
+  Δ1 ∘ Δ2 => Δ -> Δa ∘ Δb => Δ1 -> exists Δc, Δa ∘ Δ2 => Δc /\ Δc ∘ Δb => Δ.
+Proof with eauto using merge.
+  move=>mrg. elim: mrg Δa Δb=>{Δ1 Δ2 Δ}.
+  { move=>Δa Δb mrg. inv mrg. exists nil... }
+  { move=>Δ1 Δ2 Δ m mrg1 ih Δa Δb mrg2. inv mrg2.
+    have[Δc[mrga mrgb]]:=ih _ _ H2.
+    exists (m :U Δc)... }
+  { move=>Δ1 Δ2 Δ m mrg1 ih Δa Δb mrg2. inv mrg2.
+    have[Δc[mrga mrgb]]:=ih _ _ H2. exists (m :L Δc)...
+    have[Δc[mrga mrgb]]:=ih _ _ H2. exists (_: Δc)... }
+  { move=>Δ1 Δ2 Δ m mrg1 ih Δa Δb mrg2. inv mrg2.
+    have[Δc[mrga mrgb]]:=ih _ _ H2. exists (m :L Δc)... }
+  { move=>Δ1 Δ2 Δ mrg1 ih Δa Δb mrg2. inv mrg2.
+    have[Δc[mrga mrgb]]:=ih _ _ H2. exists (_: Δc)... }
+Qed.
+
+Lemma merge_splitR Δ1 Δ2 Δ Δa Δb :
+  Δ1 ∘ Δ2 => Δ -> Δa ∘ Δb => Δ1 -> exists Δc, Δb ∘ Δ2 => Δc /\ Δc ∘ Δa => Δ.
+Proof with eauto using merge.
+  move=>mrg. elim: mrg Δa Δb=>{Δ1 Δ2 Δ}.
+  { move=>Δa Δb mrg. inv mrg. exists nil... }
+  { move=>Δ1 Δ2 Δ m mrg1 ih Δa Δb mrg2. inv mrg2.
+    have[Δc[mrga mrgb]]:=ih _ _ H2.
+    exists (m :U Δc)... }
+  { move=>Δ1 Δ2 Δ m mrg1 ih Δa Δb mrg2. inv mrg2.
+    have[Δc[mrga mrgb]]:=ih _ _ H2. exists (_: Δc)...
+    have[Δc[mrga mrgb]]:=ih _ _ H2. exists (m :L Δc)... }
+  { move=>Δ1 Δ2 Δ m mrg1 ih Δa Δb mrg2. inv mrg2.
+    have[Δc[mrga mrgb]]:=ih _ _ H2. exists (m :L Δc)... }
+  { move=>Δ1 Δ2 Δ mrg1 ih Δa Δb mrg2. inv mrg2.
+    have[Δc[mrga mrgb]]:=ih _ _ H2. exists (_: Δc)... }
+Qed.
