theories/dyn_subst.v
@@ -1,40 +1,181 @@
 From mathcomp Require Import ssreflect ssrbool eqtype ssrnat seq.
 From Coq Require Import ssrfun Classical Utf8.
-Require Export AutosubstSsr ARS sta_subst dyn_weak.
+Require Export AutosubstSsr ARS sta_subst dyn_valid dyn_weak.
 
 Set Implicit Arguments.
 Unset Strict Implicit.
 Unset Printing Implicit Defensive.
 
 Reserved Notation "Γ1 ; Δ1 ⊨ σ ⫤ Γ2 ; Δ2" (at level 50, σ, Γ2 at next level).
-
 Inductive dyn_agree_subst :
-  context term -> (var -> term) -> context term -> Prop :=
-| agree_subst_nil σ :
-  nil ⊢ σ ⊣ nil
-| agree_subst_ty Δ σ Γ s A :
-  Δ ⊢ σ ⊣ Γ ->
-  A.[σ] :{s} Δ ⊢ up σ ⊣ A :{s} Γ
-| agree_subst_n Δ σ Γ :
-  Δ ⊢ σ ⊣ Γ ->
-  _: Δ ⊢ up σ ⊣ _: Γ
-| agree_subst_wkU Δ σ Γ n A :
-  Δ ⊢ σ ⊣ Γ ->
-  [Δ] ⊢ n : A.[σ] : U ->
-  Δ ⊢ n .: σ ⊣ A :U Γ
-| agree_subst_wkL Δ1 Δ2 Δ σ Γ n A :
-  Δ1 ∘ Δ2 => Δ ->
-  Δ1 ⊢ σ ⊣ Γ ->
-  Δ2 ⊢ n : A.[σ] : L ->
-  Δ ⊢ n .: σ ⊣ A :L Γ
-| agree_subst_wkN Δ σ Γ n :
-  Δ ⊢ σ ⊣ Γ ->
-  Δ ⊢ n .: σ ⊣ _: Γ
-| agree_subst_conv Δ σ Γ A B s l :
-  A <: B ->
-  [Δ] ⊢ B.[ren (+1)].[σ] : s @ l : U ->
-  [Γ] ⊢ B : s @ l : U ->
-  Δ ⊢ σ ⊣ A :{s} Γ ->
-  Δ ⊢ σ ⊣ B :{s} Γ
-where "Δ ⊢ σ ⊣ Γ" := (agree_subst Δ σ Γ).
+  sta_ctx -> dyn_ctx -> (var -> term) -> sta_ctx -> dyn_ctx -> Prop :=
+| dyn_agree_subst_nil σ :
+  nil ; nil ⊨ σ ⫤ nil ; nil
+| dyn_agree_subst_ty Γ1 Δ1 σ Γ2 Δ2 A s :
+  Γ1 ; Δ1 ⊨ σ ⫤ Γ2 ; Δ2 ->
+  (A.[σ] :: Γ1) ; (A.[σ] :{s} Δ1) ⊨ up σ ⫤ (A :: Γ2) ; (A :{s} Δ2)
+| dyn_agree_subst_n Γ1 Δ1 σ Γ2 Δ2 A :
+  Γ1 ; Δ1 ⊨ σ ⫤ Γ2 ; Δ2 ->
+  (A.[σ] :: Γ1) ; (_: Δ1) ⊨ up σ ⫤ (A :: Γ2) ; (_: Δ2)
+| dyn_agree_subst_wk0 Γ1 Δ1 σ Γ2 Δ2 n A :
+  Γ1 ; Δ1 ⊨ σ ⫤ Γ2 ; Δ2 ->
+  Γ1 ⊢ n : A.[σ] ->
+  Γ1 ; Δ1 ⊨ n .: σ ⫤ (A :: Γ2) ; (_: Δ2)
+| dyn_agree_subst_wk1 Γ1 Γ2 σ Δ1 Δ2 Δa Δb n A s :
+  Δb ▷ s ->
+  Δa ∘ Δb => Δ1 ->
+  Γ1 ; Δa ⊨ σ ⫤ Γ2 ; Δ2 ->
+  Γ1 ; Δb ⊨ n : A.[σ] ->
+  Γ1 ; Δ1 ⊨ n .: σ ⫤ (A :: Γ2) ; (A :{s} Δ2)
+| dyn_agree_subst_conv0 Γ1 Δ1 σ Γ2 Δ2 A B s :
+  A === B ->
+  Γ1 ⊢ B.[ren (+1)].[σ] : @s ->
+  Γ2 ⊢ B : @s ->
+  Γ1 ; Δ1 ⊨ σ ⫤ (A :: Γ2) ; (_: Δ2) ->
+  Γ1 ; Δ1 ⊨ σ ⫤ (B :: Γ2) ; (_: Δ2)
+| dyn_agree_subst_conv1 Γ1 Δ1 σ Γ2 Δ2 A B s :
+  A === B ->
+  Γ1 ⊢ B.[ren (+1)].[σ] : @s ->
+  Γ2 ⊢ B : @s ->
+  Γ1 ; Δ1 ⊨ σ ⫤ (A :: Γ2) ; (A :{s} Δ2) ->
+  Γ1 ; Δ1 ⊨ σ ⫤ (B :: Γ2) ; (B :{s} Δ2)
+where "Γ1 ; Δ1 ⊨ σ ⫤ Γ2 ; Δ2" := (dyn_agree_subst Γ1 Δ1 σ Γ2 Δ2).
 
+Lemma dyn_agree_subst_key Γ1 Γ2 Δ1 Δ2 σ s :
+  Γ1 ; Δ1 ⊨ σ ⫤ Γ2 ; Δ2 -> Δ2 ▷ s -> Δ1 ▷ s.
+Proof with eauto using key.
+  move=>agr. elim: agr s=>{Γ1 Γ2 Δ1 Δ2 σ}...
+  { move=>Γ1 Δ1 σ Γ2 Δ2 A s agr ih r k. inv k... }
+  { move=>Γ1 Δ1 σ Γ2 Δ2 _ agr ih s k. inv k... }
+  { move=>Γ1 Δ1 σ Γ2 Δ2 n A agr ih tyn s k. inv k... }
+  { move=>Γ1 Γ2 σ Δ1 Δ2 Δa Δb n A s k1 mrg agr ih tyn r k2. inv k2...
+    apply: key_merge...
+    apply: key_impure. }
+  { move=>Γ1 Δ1 σ Γ2 Δ2 A B s eq tyB1 tyB2 agr ih r k. inv k... }
+Qed.
+
+Lemma dyn_sta_agree_subst Γ1 Γ2 Δ1 Δ2 σ :
+  Γ1 ; Δ1 ⊨ σ ⫤ Γ2 ; Δ2 -> Γ1 ⊢ σ ⊣ Γ2.
+Proof with eauto using sta_agree_subst.
+  elim=>{Γ1 Γ2 Δ1 Δ2 σ}...
+  move=>Γ1 Γ2 σ Δ1 Δ2 Δa Δb n A s _ _ _ agr tyn.
+  constructor...
+  apply: dyn_sta_type...
+Qed.
+
+Lemma dyn_agree_subst_refl Γ Δ : dyn_wf Γ Δ -> Γ ; Δ ⊨ ids ⫤ Γ ; Δ.
+Proof with eauto using dyn_agree_subst.
+  elim: Γ Δ.
+  { move=>Δ wf. inv wf... }
+  { move=>A Γ ih Δ wf. inv wf.
+    { have agr:=ih _ H1.
+      have:(A.[ids] :: Γ); A.[ids] :{s} Δ0 ⊨ up ids ⫤ (A :: Γ); A :{s} Δ0...
+      by asimpl. }
+    { have agr:=ih _ H1.
+      have:(A.[ids] :: Γ); _: Δ0 ⊨ up ids ⫤ (A :: Γ); _: Δ0...
+      by asimpl. } }
+Qed.
+
+Lemma dyn_wf_merge Γ Δ Δ1 Δ2 :
+  Δ1 ∘ Δ2 => Δ -> dyn_wf Γ Δ -> dyn_wf Γ Δ1 /\ dyn_wf Γ Δ2.
+Proof with eauto using dyn_wf.
+  move=>mrg agr. elim: agr Δ1 Δ2 mrg=>{Γ Δ}.
+  { move=>Δ1 Δ2 mrg. inv mrg... }
+  { move=>Γ Δ A s wf ih tyA Δ1 Δ2 mrg. inv mrg.
+    { have[wf1 wf2]:=ih _ _ H2... }
+    { have[wf1 wf2]:=ih _ _ H2... }
+    { have[wf1 wf2]:=ih _ _ H2... } }
+  { move=>Γ Δ A s wf ih tyA Δ1 Δ2 mrg. inv mrg.
+    have[wf1 wf2]:=ih _ _ H2... }
+Qed.
+
+Lemma dyn_agree_subst_has Γ1 Γ2 σ Δ1 Δ2 x A :
+  dyn_wf Γ1 Δ1 ->
+  Γ1 ; Δ1 ⊨ σ ⫤ Γ2 ; Δ2 -> dyn_has Δ2 x A -> Γ1 ; Δ1 ⊨ (σ x) : A.[σ].
+Proof with eauto using dyn_agree_subst, dyn_agree_subst_key.
+  move=>wf agr. elim: agr wf x A=>{Γ1 Γ2 σ Δ1 Δ2}...
+  { move=>σ _ x A hs. inv hs. }
+  { move=>Γ1 Δ1 σ Γ2 Δ2 A s agr ih wf x B hs.
+    inv wf. inv hs; asimpl.
+    replace A.[σ >> ren (+1)] with A.[σ].[ren (+1)] by autosubst.
+    apply: dyn_var; constructor...
+    replace A0.[σ >> ren (+1)] with A0.[σ].[ren (+1)] by autosubst.
+    apply: dyn_eweakenU... }
+  { move=>Γ1 Δ1 σ Γ2 Δ2 A agr ih wf x B hs.
+    inv wf. inv hs; asimpl...
+    replace A0.[σ >> ren (+1)] with A0.[σ].[ren (+1)]
+      by autosubst.
+    apply: dyn_eweakenN... }
+  { move=>Γ1 Δ1 σ Γ2 Δ2 n A agr ih tyn wf x B hs. inv hs; asimpl... }
+  { move=>Γ1 Γ2 σ Δ1 Δ2 Δa Δb n A s k mrg agr ih tyn wf x B hs.
+    inv hs; asimpl.
+    { have ka:=dyn_agree_subst_key agr H4.
+      have->//:=merge_pureL mrg ka. }
+    { have->:=merge_pureR mrg k.
+      apply: ih...
+      have[]//:=dyn_wf_merge mrg wf. } }
+  { move=>Γ1 Δ1 σ Γ2 Δ2 A B s eq tyB1 tyB2 agr ih wf x C hs. inv hs.
+    { apply: dyn_conv.
+      apply: sta_conv_subst.
+      apply: sta_conv_subst...
+      apply: ih...
+      constructor...
+      exact: tyB1. }
+    { apply: ih...
+      constructor... } }
+Qed.
+
+Lemma dyn_agree_subst_merge Γ1 Γ2 Δ1 Δ2 Δa Δb σ :
+  Γ1 ; Δ1 ⊨ σ ⫤ Γ2 ; Δ2 -> Δa ∘ Δb => Δ2 ->
+  exists Δa' Δb',
+    Δa' ∘ Δb' => Δ1 /\ Γ1 ; Δa' ⊨ σ ⫤ Γ2 ; Δa /\ Γ1 ; Δb' ⊨ σ ⫤ Γ2 ; Δb.
+Proof with eauto 6 using merge, dyn_agree_subst, dyn_agree_subst_key.
+  move=>agr. elim: agr Δa Δb=>{Γ1 Γ2 Δ1 Δ2 σ}.
+  { move=>σ Δa Δb mrg. inv mrg.
+    exists nil. exists nil... }
+  { move=>Γ1 Δ1 σ Γ2 Δ2 A s agr ih Δa Δb mrg. inv mrg.
+    { have[Δa[Δb[mrg[agra agrb]]]]:=ih _ _ H2.
+      exists (A.[σ] :U Δa). exists (A.[σ] :U Δb)... }
+    { have[Δa[Δb[mrg[agra agrb]]]]:=ih _ _ H2.
+      exists (A.[σ] :L Δa). exists (_: Δb)... }
+    { have[Δa[Δb[mrg[agra agrb]]]]:=ih _ _ H2.
+      exists (_: Δa). exists (A.[σ] :L Δb)... } }
+  { move=>Γ1 Δ1 σ Γ2 Δ2 A agr ih Δa Δb mrg. inv mrg.
+    have[Δa[Δb[mrg[agra agrb]]]]:=ih _ _ H2.
+    exists (_: Δa). exists (_: Δb)... }
+  { move=>Γ1 Δ1 σ Γ2 Δ2 n A agr ih tyn Δa Δb mrg. inv mrg.
+    have[Δa[Δb[mrg[agra agrb]]]]:=ih _ _ H2.
+    exists Δa. exists Δb... }
+  { move=>Γ1 Γ2 σ Δ1 Δ2 Δa Δb n A s k mrg agr ih tyn Δa' Δb' mrg'. inv mrg'.
+    { have[Δa'[Δb'[mrg'[agra agrb]]]]:=ih _ _ H2.
+      have[Δc[mrg1 mrg2]]:=merge_splitL mrg mrg'.
+      exists Δc. exists Δb'.
+      repeat split...
+      apply: dyn_agree_subst_wk1...
+      have[Δd[mrg3 mrg4]]:=merge_splitR mrg mrg'.
+      have e:=merge_pureR mrg3 k.
+      by subst. }
+    { have[Δa'[Δb'[mrg'[agra agrb]]]]:=ih _ _ H2.
+      have[Δc[mrg1 mrg2]]:=merge_splitL mrg mrg'.
+      exists Δc. exists Δb'.
+      repeat split...
+      apply: dyn_agree_subst_wk0...
+      apply: dyn_sta_type... }
+    { have[Δa'[Δb'[mrg'[agra agrb]]]]:=ih _ _ H2.
+      have[Δc[mrg1 mrg2]]:=merge_splitR mrg mrg'.
+      exists Δa'. exists Δc.
+      repeat split...
+      exact: merge_sym.
+      apply: dyn_agree_subst_wk0...
+      apply: dyn_sta_type... } }
+  { move=>Γ1 Δ1 σ Γ2 Δ2 A B s eq tyB1 tyB2 agr ih Δa Δb mrg. inv mrg.
+    have[Δa'[Δb'[mrg'[agra agrb]]]]:=ih _ _ (merge_null H2).
+    exists Δa'. exists Δb'... }
+  { move=>Γ1 Δ1 σ Γ2 Δ2 A B s eq tyB1 tyB2 agr ih Δa Δb mrg. inv mrg.
+    { have[Δa'[Δb'[mrg'[agra agrb]]]]:=ih _ _ (merge_left A H2).
+      exists Δa'. exists Δb'... }
+    { have[Δa'[Δb'[mrg'[agra agrb]]]]:=ih _ _ (merge_right1 A H2).
+      exists Δa'. exists Δb'... }
+    { have[Δa'[Δb'[mrg'[agra agrb]]]]:=ih _ _ (merge_right2 A H2).
+      exists Δa'. exists Δb'... } }
+Qed.
